

HW3

[2-3] 3

$$3. f(x) = x^{75} - x + 3 \Rightarrow f'(x) = 75x^{75-1} - 1(1) + 0 = 75x^{74} - 1$$

[2-3] 7

$$7. f(x) = x^{3/2} + x^{-3} \Rightarrow f'(x) = \frac{3}{2}x^{1/2} + (-3x^{-4}) = \frac{3}{2}x^{1/2} - 3x^{-4}$$

[2-3] 13

$$13. g(x) = \frac{1}{\sqrt{x}} + \sqrt[4]{x} = x^{-1/2} + x^{1/4} \Rightarrow g'(x) = -\frac{1}{2}x^{-3/2} + \frac{1}{4}x^{-3/4} \text{ or } -\frac{1}{2x\sqrt{x}} + \frac{1}{4\sqrt[4]{x^3}}$$

[2-3] 26

$$26. y = \frac{t}{x^2} + \frac{x}{t} = tx^{-2} + xt^{-1}.$$

To find dy/dx , we treat t as a constant and x as a variable to get $dy/dx = t(-2x^{-3}) + (1)t^{-1} = -2tx^{-3} + t^{-1}$ or

$$-\frac{2t}{x^3} + \frac{1}{t}.$$

To find dy/dt , we treat x as a constant and t as a variable to get $dy/dt = (1)x^{-2} + x(-1t^{-2}) = x^{-2} - xt^{-2}$ or $\frac{1}{x^2} - \frac{x}{t^2}$.

[2-3] 30

$$30. \text{ By the Product Rule, } y = (10x^2 + 7x - 2)(2 - x^2) \Rightarrow$$

$$\begin{aligned} y' &= (10x^2 + 7x - 2)(2 - x^2)' + (2 - x^2)(10x^2 + 7x - 2)' = (10x^2 + 7x - 2)(-2x) + (2 - x^2)(20x + 7) \\ &= -20x^3 - 14x^2 + 4x + 40x + 14 - 20x^3 - 7x^2 = -40x^3 - 21x^2 + 44x + 14 \end{aligned}$$

[2-3] 33

33. By the Quotient Rule, $y = \frac{5x}{1+x} \Rightarrow$

$$y' = \frac{(1+x)(5x)' - 5x(1+x)'}{(1+x)^2} = \frac{(1+x)5 - 5x(1)}{(1+x)^2} = \frac{5 + 5x - 5x}{(1+x)^2} = \frac{5}{(1+x)^2}.$$

[2-3] 45

$$45. J(u) = \left(\frac{1}{u} + \frac{1}{u^2}\right)\left(u + \frac{1}{u}\right) = (u^{-1} + u^{-2})(u + u^{-1}) \xRightarrow{\text{PR}}$$

$$\begin{aligned} J'(u) &= (u^{-1} + u^{-2})(u + u^{-1})' + (u + u^{-1})(u^{-1} + u^{-2})' = (u^{-1} + u^{-2})(1 - u^{-2}) + (u + u^{-1})(-u^{-2} - 2u^{-3}) \\ &= u^{-1} - u^{-3} + u^{-2} - u^{-4} - u^{-1} - 2u^{-2} - u^{-3} - 2u^{-4} = -u^{-2} - 2u^{-3} - 3u^{-4} = -\left(\frac{1}{u^2} + \frac{2}{u^3} + \frac{3}{u^4}\right) \end{aligned}$$

[2-3] 59

$$59. y = \frac{2x}{x+1} \Rightarrow y' = \frac{(x+1)(2) - (2x)(1)}{(x+1)^2} = \frac{2}{(x+1)^2}.$$

At $(1, 1)$, $y' = \frac{1}{2}$, and an equation of the tangent line is $y - 1 = \frac{1}{2}(x - 1)$, or $y = \frac{1}{2}x + \frac{1}{2}$.

[2-4] 1

$$1. f(x) = 3 \sin x - 2 \cos x \Rightarrow f'(x) = 3(\cos x) - 2(-\sin x) = 3 \cos x + 2 \sin x$$

[2-4] 7

$$7. y = \sec \theta \tan \theta \Rightarrow y' = \sec \theta (\sec^2 \theta) + \tan \theta (\sec \theta \tan \theta) = \sec \theta (\sec^2 \theta + \tan^2 \theta). \text{ Using the identity}$$

$1 + \tan^2 \theta = \sec^2 \theta$, we can write alternative forms of the answer as $\sec \theta (1 + 2 \tan^2 \theta)$ or $\sec \theta (2 \sec^2 \theta - 1)$.

[2-4] 15

$$15. y = \frac{x}{2 - \tan x} \Rightarrow y' = \frac{(2 - \tan x)(1) - x(-\sec^2 x)}{(2 - \tan x)^2} = \frac{2 - \tan x + x \sec^2 x}{(2 - \tan x)^2}$$

[2-4] 24

$$24. \frac{d}{dx}(\sec x) = \frac{d}{dx} \left(\frac{1}{\cos x} \right) = \frac{(\cos x)(0) - 1(-\sin x)}{\cos^2 x} = \frac{\sin x}{\cos^2 x} = \frac{1}{\cos x} \cdot \frac{\sin x}{\cos x} = \sec x \tan x$$

[2-4] 35

$$35. g(\theta) = \frac{\sin \theta}{\theta} \xRightarrow{\text{QR}} g'(\theta) = \frac{\theta(\cos \theta) - (\sin \theta)(1)}{\theta^2} = \frac{\theta \cos \theta - \sin \theta}{\theta^2}$$

Using the Quotient Rule and $g'(\theta) = \frac{\theta \cos \theta - \sin \theta}{\theta^2}$, we get

$$\begin{aligned} g''(\theta) &= \frac{\theta^2 \{ [\theta(-\sin \theta) + (\cos \theta)(1)] - \cos \theta \} - (\theta \cos \theta - \sin \theta)(2\theta)}{(\theta^2)^2} \\ &= \frac{-\theta^3 \sin \theta + \theta^2 \cos \theta - \theta^2 \cos \theta - 2\theta^2 \cos \theta + 2\theta \sin \theta}{\theta^4} = \frac{\theta(-\theta^2 \sin \theta - 2\theta \cos \theta + 2 \sin \theta)}{\theta \cdot \theta^3} \\ &= \frac{-\theta^2 \sin \theta - 2\theta \cos \theta + 2 \sin \theta}{\theta^3} \end{aligned}$$

[2-4] 45

$$45. \lim_{x \rightarrow 0} \frac{\sin 5x}{3x} = \lim_{x \rightarrow 0} \frac{5}{3} \left(\frac{\sin 5x}{5x} \right) = \frac{5}{3} \lim_{x \rightarrow 0} \frac{\sin 5x}{5x} = \frac{5}{3} \lim_{\theta \rightarrow 0} \frac{\sin \theta}{\theta} \quad \left[\begin{array}{l} \text{where } \theta = 5x, \\ \text{using Equation 5} \end{array} \right] = \frac{5}{3} \cdot 1 = \frac{5}{3}$$

[2-4] 51

$$\begin{aligned}
 51. \quad \lim_{x \rightarrow 0} \frac{\tan 2x}{x} &= \lim_{x \rightarrow 0} \frac{\frac{\sin 2x}{\cos 2x}}{x} = \lim_{x \rightarrow 0} \frac{\sin 2x}{x \cos 2x} = \lim_{x \rightarrow 0} \frac{\sin 2x}{2x} \cdot \frac{2}{\cos 2x} \\
 &= \lim_{x \rightarrow 0} \frac{\sin 2x}{2x} \cdot \lim_{x \rightarrow 0} \frac{2}{\cos 2x} = \lim_{x \rightarrow 0} \frac{\sin \theta}{\theta} \cdot \lim_{x \rightarrow 0} \frac{2}{\cos 2x} \quad [\theta = 2x] \\
 &= 1 \cdot \frac{2}{1} = 2
 \end{aligned}$$

[2-4] 62

62. Let $f(x) = x \sin x$ and $h(x) = \sin x$, so $f(x) = xh(x)$. Then $f'(x) = h(x) + xh'(x)$,

$$f''(x) = h'(x) + h'(x) + xh''(x) = 2h'(x) + xh''(x),$$

$$f'''(x) = 2h''(x) + h''(x) + xh'''(x) = 3h''(x) + xh'''(x), \dots, f^{(n)}(x) = nh^{(n-1)}(x) + xh^{(n)}(x).$$

Since $34 = 4(8) + 2$, we have $h^{(34)}(x) = h^{(2)}(x) = \frac{d^2}{dx^2}(\sin x) = -\sin x$ and $h^{(35)}(x) = -\cos x$.

$$\text{Thus, } \frac{d^{35}}{dx^{35}}(x \sin x) = 35h^{(34)}(x) + xh^{(35)}(x) = -35 \sin x - x \cos x.$$

[2-5] 3

3. Let $u = g(x) = \cos x$ and $y = f(u) = \sin u$. Then

$$\frac{dy}{dx} = \frac{dy}{du} \frac{du}{dx} = (\cos u)(-\sin x) = (\cos(\cos x))(-\sin x) = -\sin x \cos(\cos x).$$

[2-5] 6

$$6. \text{ Let } u = g(x) = \sqrt{x} \text{ and } y = f(u) = \sin u. \text{ Then } \frac{dy}{dx} = \frac{dy}{du} \frac{du}{dx} = (\cos u) \left(\frac{1}{2} x^{-1/2} \right) = \frac{\cos u}{2\sqrt{x}} = \frac{\cos \sqrt{x}}{2\sqrt{x}}.$$

[2-5] 18

$$18. \text{ Using the Product Rule and the Chain Rule, } f(t) = t \sin \pi t \Rightarrow f'(t) = t(\cos \pi t) \cdot \pi + (\sin \pi t) \cdot 1 = \pi t \cos \pi t + \sin \pi t.$$

[2-5] 29

29. $y = \cos(\sec 4x) \Rightarrow$

$$y' = -\sin(\sec 4x) \frac{d}{dx} \sec 4x = -\sin(\sec 4x) \cdot \sec 4x \tan 4x \cdot 4 = -4 \sin(\sec 4x) \sec 4x \tan 4x$$